Except additional exercise

Imp.v
@@ -410,3 +410,446 @@ Inductive aevalR : aexp -> nat -> Prop :=
 where "a '||' n" := (aevalR a n) : type_scope.
 
 End aevalR_extended.
+
+Module Id.
+
+Inductive id : Type :=
+  Id : nat -> id.
+
+Theorem eq_id_dec : forall id1 id2 : id, {id1 = id2} + {id1 <> id2}.
+Proof.
+   intros id1 id2.
+   destruct id1 as [n1]. destruct id2 as [n2].
+   destruct (eq_nat_dec n1 n2) as [Heq | Hneq].
+   Case "n1 = n2".
+     left. rewrite Heq. reflexivity.
+   Case "n1 <> n2".
+     right. intros contra. inversion contra. apply Hneq. apply H0.
+Defined.
+
+Lemma eq_id : forall (T:Type) x (p q:T),
+              (if eq_id_dec x x then p else q) = p.
+Proof.
+  intros.
+  destruct (eq_id_dec x x).
+  Case "x = x".
+    reflexivity.
+  Case "x <> x (impossible)".
+    apply ex_falso_quodlibet; apply n; reflexivity. Qed.
+
+(* Exercise: 1 star, optional (neq_id) *)
+
+Lemma neq_id : forall (T:Type) x y (p q:T), x <> y ->
+               (if eq_id_dec x y then p else q) = q.
+Proof.
+  intros.
+  destruct (eq_id_dec x y).
+  Case "x = y". apply ex_falso_quodlibet; apply H; apply e.
+  Case "x <> y". reflexivity.
+Qed.
+
+Definition state := id -> nat.
+
+Definition empty_state : state :=
+  fun _ => 0.
+
+Definition update (st : state) (x : id) (n : nat) : state :=
+  fun x' => if eq_id_dec x x' then n else st x'.
+
+(* Exercise: 1 star (update_eq) *)
+
+Theorem update_eq : forall n x st,
+  (update st x n) x = n.
+Proof.
+  intros. unfold update. apply eq_id.
+Qed.
+
+(* Exercise: 1 star (update_neq) *)
+
+Theorem update_neq : forall x2 x1 n st,
+  x2 <> x1 ->
+  (update st x2 n) x1 = (st x1).
+Proof.
+  intros. unfold update. apply neq_id. apply H. Qed.
+
+(* Exercise: 1 star (update_example) *)
+
+Theorem update_example : forall (n:nat),
+  (update empty_state (Id 2) n) (Id 3) = 0.
+Proof.
+  intros. unfold update.
+  apply neq_id. intros contra. inversion contra.
+Qed.
+
+(* Exercise: 1 star (update_shadow) *)
+
+Theorem update_shadow : forall n1 n2 x1 x2 (st : state),
+   (update  (update st x2 n1) x2 n2) x1 = (update st x2 n2) x1.
+Proof.
+  intros.
+  unfold update. destruct (eq_id_dec x2 x1); reflexivity.
+Qed.
+
+(* Exercise: 2 stars (update_same) *)
+
+Theorem update_same : forall n1 x1 x2 (st : state),
+  st x1 = n1 ->
+  (update st x1 n1) x2 = st x2.
+Proof.
+  intros. unfold update. destruct (eq_id_dec x1 x2). subst. reflexivity.
+  reflexivity.
+Qed.
+
+(* Exercise: 3 stars (update_permute) *)
+Theorem update_permute : forall n1 n2 x1 x2 x3 st,
+  x2 <> x1 ->
+  (update (update st x2 n1) x1 n2) x3 = (update (update st x1 n2) x2 n1) x3.
+Proof.
+  intros. unfold update.
+  destruct (eq_id_dec x1 x3) eqn: x1x3.
+    destruct (eq_id_dec x2 x3) eqn: x2x3.
+      apply ex_falso_quodlibet. apply H. subst. reflexivity.
+      reflexivity.
+    destruct (eq_id_dec x2 x3) eqn: x2x3; reflexivity.
+Qed.
+
+Inductive aexp : Type :=
+  | ANum : nat -> aexp
+  | AId : id -> aexp                (* <----- NEW *)
+  | APlus : aexp -> aexp -> aexp
+  | AMinus : aexp -> aexp -> aexp
+  | AMult : aexp -> aexp -> aexp.
+
+Tactic Notation "aexp_cases" tactic(first) ident(c) :=
+  first;
+  [ Case_aux c "ANum" | Case_aux c "AId" | Case_aux c "APlus"
+  | Case_aux c "AMinus" | Case_aux c "AMult" ].
+
+Definition X : id := Id 0.
+Definition Y : id := Id 1.
+Definition Z : id := Id 2.
+
+Inductive bexp : Type :=
+  | BTrue : bexp
+  | BFalse : bexp
+  | BEq : aexp -> aexp -> bexp
+  | BLe : aexp -> aexp -> bexp
+  | BNot : bexp -> bexp
+  | BAnd : bexp -> bexp -> bexp.
+
+Tactic Notation "bexp_cases" tactic(first) ident(c) :=
+  first;
+  [ Case_aux c "BTrue" | Case_aux c "BFalse" | Case_aux c "BEq"
+  | Case_aux c "BLe" | Case_aux c "BNot" | Case_aux c "BAnd" ].
+
+Fixpoint aeval (st : state) (a : aexp) : nat :=
+  match a with
+  | ANum n => n
+  | AId x => st x                                        (* <----- NEW *)
+  | APlus a1 a2 => (aeval st a1) + (aeval st a2)
+  | AMinus a1 a2  => (aeval st a1) - (aeval st a2)
+  | AMult a1 a2 => (aeval st a1) * (aeval st a2)
+  end.
+
+Fixpoint beval (st : state) (b : bexp) : bool :=
+  match b with
+  | BTrue       => true
+  | BFalse      => false
+  | BEq a1 a2   => beq_nat (aeval st a1) (aeval st a2)
+  | BLe a1 a2   => ble_nat (aeval st a1) (aeval st a2)
+  | BNot b1     => negb (beval st b1)
+  | BAnd b1 b2  => andb (beval st b1) (beval st b2)
+  end.
+
+Example aexp1 :
+  aeval (update empty_state X 5)
+        (APlus (ANum 3) (AMult (AId X) (ANum 2)))
+  = 13.
+Proof. reflexivity. Qed.
+
+Example bexp1 :
+  beval (update empty_state X 5)
+        (BAnd BTrue (BNot (BLe (AId X) (ANum 4))))
+  = true.
+Proof. reflexivity. Qed.
+
+(* Commands *)
+
+Inductive com : Type :=
+  | CSkip : com
+  | CAss : id -> aexp -> com
+  | CSeq : com -> com -> com
+  | CIf : bexp -> com -> com -> com
+  | CWhile : bexp -> com -> com.
+
+Tactic Notation "com_cases" tactic(first) ident(c) :=
+  first;
+  [ Case_aux c "SKIP" | Case_aux c "::=" | Case_aux c ";;"
+  | Case_aux c "IFB" | Case_aux c "WHILE" ].
+
+Notation "'SKIP'" :=
+  CSkip.
+Notation "x '::=' a" :=
+  (CAss x a) (at level 60).
+Notation "c1 ;; c2" :=
+  (CSeq c1 c2) (at level 80, right associativity).
+Notation "'WHILE' b 'DO' c 'END'" :=
+  (CWhile b c) (at level 80, right associativity).
+Notation "'IFB' c1 'THEN' c2 'ELSE' c3 'FI'" :=
+  (CIf c1 c2 c3) (at level 80, right associativity).
+
+Definition fact_in_coq : com :=
+  Z ::= AId X;;
+  Y ::= ANum 1;;
+  WHILE BNot (BEq (AId Z) (ANum 0)) DO
+    Y ::= AMult (AId Y) (AId Z);;
+    Z ::= AMinus (AId Z) (ANum 1)
+  END.
+
+Definition plus2 : com :=
+  X ::= (APlus (AId X) (ANum 2)).
+
+Definition XtimesYinZ : com :=
+  Z ::= (AMult (AId X) (AId Y)).
+
+Definition subtract_slowly_body : com :=
+  Z ::= AMinus (AId Z) (ANum 1) ;;
+  X ::= AMinus (AId X) (ANum 1).
+
+Definition subtract_slowly : com :=
+  WHILE BNot (BEq (AId X) (ANum 0)) DO
+    subtract_slowly_body
+  END.
+
+Definition subtract_3_from_5_slowly : com :=
+  X ::= ANum 3 ;;
+  Z ::= ANum 5 ;;
+  subtract_slowly.
+
+Definition loop : com :=
+  WHILE BTrue DO
+    SKIP
+  END.
+
+(* Evaluation *)
+
+Fixpoint ceval_fun_no_while (st : state) (c : com) : state :=
+  match c with
+    | SKIP =>
+        st
+    | x ::= a1 =>
+        update st x (aeval st a1)
+    | c1 ;; c2 =>
+        let st' := ceval_fun_no_while st c1 in
+        ceval_fun_no_while st' c2
+    | IFB b THEN c1 ELSE c2 FI =>
+        if (beval st b)
+          then ceval_fun_no_while st c1
+          else ceval_fun_no_while st c2
+    | WHILE b DO c END =>
+        st  (* bogus *)
+  end.
+
+Reserved Notation "c1 '/' st '||' st'" (at level 40, st at level 39).
+
+Inductive ceval : com -> state -> state -> Prop :=
+  | E_Skip : forall st,
+      SKIP / st || st
+  | E_Ass  : forall st a1 n x,
+      aeval st a1 = n ->
+      (x ::= a1) / st || (update st x n)
+  | E_Seq : forall c1 c2 st st' st'',
+      c1 / st  || st' ->
+      c2 / st' || st'' ->
+      (c1 ;; c2) / st || st''
+  | E_IfTrue : forall st st' b c1 c2,
+      beval st b = true ->
+      c1 / st || st' ->
+      (IFB b THEN c1 ELSE c2 FI) / st || st'
+  | E_IfFalse : forall st st' b c1 c2,
+      beval st b = false ->
+      c2 / st || st' ->
+      (IFB b THEN c1 ELSE c2 FI) / st || st'
+  | E_WhileEnd : forall b st c,
+      beval st b = false ->
+      (WHILE b DO c END) / st || st
+  | E_WhileLoop : forall st st' st'' b c,
+      beval st b = true ->
+      c / st || st' ->
+      (WHILE b DO c END) / st' || st'' ->
+      (WHILE b DO c END) / st || st''
+
+  where "c1 '/' st '||' st'" := (ceval c1 st st').
+
+Tactic Notation "ceval_cases" tactic(first) ident(c) :=
+  first;
+  [ Case_aux c "E_Skip" | Case_aux c "E_Ass" | Case_aux c "E_Seq"
+  | Case_aux c "E_IfTrue" | Case_aux c "E_IfFalse"
+  | Case_aux c "E_WhileEnd" | Case_aux c "E_WhileLoop" ].
+
+Example ceval_example1:
+    (X ::= ANum 2;;
+     IFB BLe (AId X) (ANum 1)
+       THEN Y ::= ANum 3
+       ELSE Z ::= ANum 4
+     FI)
+   / empty_state
+   || (update (update empty_state X 2) Z 4).
+Proof.
+  (* We must supply the intermediate state *)
+  apply E_Seq with (update empty_state X 2).
+  Case "assignment command".
+    apply E_Ass. reflexivity.
+  Case "if command".
+    apply E_IfFalse.
+      reflexivity.
+      apply E_Ass. reflexivity.  Qed.
+
+(* Exercise: 2 stars (ceval_example2) *)
+
+Example ceval_example2:
+    (X ::= ANum 0;; Y ::= ANum 1;; Z ::= ANum 2) / empty_state ||
+    (update (update (update empty_state X 0) Y 1) Z 2).
+Proof.
+  apply E_Seq with (update empty_state X 0).
+  apply E_Ass. reflexivity.
+  apply E_Seq with (update (update empty_state X 0) Y 1).
+  apply E_Ass. reflexivity.
+  apply E_Ass. reflexivity.
+Qed.
+
+(* Exercise: 3 stars, advanced (pup_to_n) *)
+
+Definition pup_to_n : com :=
+  Y ::= ANum 0;;
+  WHILE (BLe (ANum 1) (AId X)) DO
+    Y ::= APlus (AId Y) (AId X);;
+    X ::= AMinus (AId X) (ANum 1)
+  END.
+
+Theorem pup_to_2_ceval :
+  pup_to_n / (update empty_state X 2) ||
+    update (update (update (update (update (update empty_state
+      X 2) Y 0) Y 2) X 1) Y 3) X 0.
+Proof.
+  unfold pup_to_n.
+  apply E_Seq with (st':= (update (update empty_state X 2) Y 0)).
+    apply E_Ass. reflexivity.
+    apply E_WhileLoop with (update (update (update (update empty_state X 2) Y 0) Y 2) X 1).
+    reflexivity. apply E_Seq with (update (update (update empty_state X 2) Y 0) Y 2); try(apply E_Ass; reflexivity).
+    apply E_WhileLoop with (update (update (update (update (update (update empty_state X 2) Y 0) Y 2) X 1) Y 3) X 0).
+    reflexivity. apply E_Seq with (update (update (update (update (update empty_state X 2) Y 0) Y 2) X 1) Y 3); try(apply E_Ass; reflexivity).
+    apply E_WhileEnd. reflexivity.
+Qed.
+
+Theorem ceval_deterministic: forall c st st1 st2,
+     c / st || st1  ->
+     c / st || st2 ->
+     st1 = st2.
+Proof.
+  intros c st st1 st2 E1 E2.
+  generalize dependent st2.
+  ceval_cases (induction E1) Case;
+           intros st2 E2; inversion E2; subst.
+  Case "E_Skip". reflexivity.
+  Case "E_Ass". reflexivity.
+  Case "E_Seq".
+    assert (st' = st'0) as EQ1.
+      SCase "Proof of assertion". apply IHE1_1; assumption.
+    subst st'0.
+    apply IHE1_2. assumption.
+  Case "E_IfTrue".
+    SCase "b1 evaluates to true".
+      apply IHE1. assumption.
+    SCase "b1 evaluates to false (contradiction)".
+      rewrite H in H5. inversion H5.
+  Case "E_IfFalse".
+    SCase "b1 evaluates to true (contradiction)".
+      rewrite H in H5. inversion H5.
+    SCase "b1 evaluates to false".
+      apply IHE1. assumption.
+  Case "E_WhileEnd".
+    SCase "b1 evaluates to false".
+      reflexivity.
+    SCase "b1 evaluates to true (contradiction)".
+      rewrite H in H2. inversion H2.
+  Case "E_WhileLoop".
+    SCase "b1 evaluates to false (contradiction)".
+      rewrite H in H4. inversion H4.
+    SCase "b1 evaluates to true".
+      assert (st' = st'0) as EQ1.
+        SSCase "Proof of assertion". apply IHE1_1; assumption.
+      subst st'0.
+      apply IHE1_2. assumption.  Qed.
+
+(* Reasoning About Imp Programs *)
+
+Theorem plus2_spec : forall st n st',
+  st X = n ->
+  plus2 / st || st' ->
+  st' X = n + 2.
+Proof.
+  intros st n st' HX Heval.
+  (* Inverting Heval essentially forces Coq to expand one
+     step of the ceval computation - in this case revealing
+     that st' must be st extended with the new value of X,
+     since plus2 is an assignment *)
+  inversion Heval. subst. clear Heval. simpl.
+  apply update_eq.  Qed.
+
+(* Exercise: 3 stars (XtimesYinZ_spec) *)
+
+Theorem XtimesYinZ_spec : forall st x y st',
+    st X = x ->
+    st Y = y ->
+    XtimesYinZ / st || st' ->
+    st' Z = x * y.
+Proof.
+  intros.
+  inversion H1. subst. simpl. apply update_eq. Qed.
+
+(* Exercise: 3 stars (loop_never_stops) *)
+
+Theorem loop_never_stops : forall st st',
+  ~(loop / st || st').
+Proof.
+  intros st st' contra. unfold loop in contra.
+  remember (WHILE BTrue DO SKIP END) as loopdef eqn:Heqloopdef.
+    (* Proceed by induction on the assumed derivation showing that
+     [loopdef] terminates.  Most of the cases are immediately
+     contradictory (and so can be solved in one step with
+     [inversion]). *)
+  induction contra; try(inversion Heqloopdef).
+  subst. inversion H.
+  subst. apply IHcontra2. reflexivity.
+Qed.
+
+(* Exercise: 3 stars (no_whilesR) *)
+
+Fixpoint no_whiles (c : com) : bool := match c with
+  | SKIP       => true
+  | _ ::= _    => true
+  | c1 ;; c2  => andb (no_whiles c1) (no_whiles c2)
+  | IFB _ THEN ct ELSE cf FI => andb (no_whiles ct) (no_whiles cf)
+  | WHILE _ DO _ END  => false
+  end.
+
+Inductive no_whilesR: com -> Prop :=
+  | NWSkip : no_whilesR SKIP
+  | NWAss : forall x e, no_whilesR (x ::= e)
+  | NWSeq : forall e1 e2, no_whilesR e1 -> no_whilesR e2 -> no_whilesR (e1 ;; e2)
+  | NWIf : forall b e1 e2, no_whilesR e1 -> no_whilesR e2 -> no_whilesR (IFB b THEN e1 ELSE e2 FI)
+  .
+
+Theorem no_whiles_eqv:
+   forall c, no_whiles c = true <-> no_whilesR c.
+Proof.
+  split.
+  Case "->".
+    intros. induction c; try(constructor);
+    try(inversion H; apply IHc1; apply andb_true_elim1 in H1; assumption);
+    try(inversion H; apply IHc2; apply andb_true_elim2 in H1; assumption).
+  Case "<-".
+    intros. induction H; try(reflexivity);
+    try(simpl; rewrite IHno_whilesR1; rewrite IHno_whilesR2; reflexivity).
+Qed.
